remove pat_tag_shift
also fix proofs for other minor updates to pat_to_clos

compiler1/semantics/closSemScript.sml
@@ -33,7 +33,7 @@ val get_global_def = Define `
     if n < LENGTH globals then SOME (EL n globals) else NONE`
 
 val Boolv_def = Define `
-  (Boolv b = Block ((if b then true_tag else false_tag)+pat_tag_shift) [])`;
+  (Boolv b = Block (if b then true_tag else false_tag) [])`;
 
 val do_eq_def = tDefine "do_eq" `
   (do_eq x y =
@@ -70,9 +70,9 @@ val do_eq_def = tDefine "do_eq" `
 
 val v_to_list_def = Define`
   (v_to_list (Block tag []) =
-     if tag = nil_tag+pat_tag_shift then SOME [] else NONE) ∧
+     if tag = nil_tag then SOME [] else NONE) ∧
   (v_to_list (Block tag [h;bt]) =
-     if tag = cons_tag+pat_tag_shift then
+     if tag = cons_tag then
        (case v_to_list bt of
         | SOME t => SOME (h::t)
         | _ => NONE )
@@ -80,11 +80,11 @@ val v_to_list_def = Define`
   (v_to_list _ = NONE)`
 
 val list_to_v_def = Define`
-  (list_to_v [] = Block (nil_tag+pat_tag_shift) []) ∧
-  (list_to_v (h::t) = Block (cons_tag+pat_tag_shift) [h;list_to_v t])`
+  (list_to_v [] = Block nil_tag []) ∧
+  (list_to_v (h::t) = Block cons_tag [h;list_to_v t])`
 
 val Unit_def = Define`
-  Unit = Block (tuple_tag+pat_tag_shift) []`
+  Unit = Block tuple_tag []`
 
 val _ = Parse.temp_overload_on("Error",``(Rerr(Rabort Rtype_error)):(closSem$v#closSem$state,closSem$v)result``)
 
@@ -159,7 +159,7 @@ val do_app_def = Define `
     | (Equal,[x1;x2]) =>
         (case do_eq x1 x2 of
          | Eq_val b => Rval (Boolv b, s)
-         | Eq_closure => Rerr (Rraise (Block (eq_tag+pat_tag_shift) []))
+         | Eq_closure => Rerr (Rraise (Block eq_tag []))
          | _ => Error)
     | (Ref,xs) =>
         let ptr = (LEAST ptr. ~(ptr IN FDOM s.refs)) in
