compiler1/pat_to_closScript.sml
@@ -4,11 +4,11 @@ val _ = new_theory"pat_to_clos"
 
 val string_tag_def = Define`string_tag = 0:num`
 val vector_tag_def = Define`vector_tag = 1:num`
-val pat_tag_shift_def = Define`pat_tag_shift = 2:num`
-(* TODO: remove pat_tag_shift - is it unnecessary? *)
 
-(* TODO: is patLang even necessary, or should it just be closLang already?
-         - yes it is necessary for Raise in Div, for example
+(* The translation from patLang to closLang is very simple.
+   Its main purpose is simplifying the semantics of some operations,
+   for example to explicitly raise an exception for Div so the semantics
+   in closLang can make more assumptions about the arguments.
 *)
 
 val compile_def = tDefine"compile"`
@@ -25,7 +25,7 @@ val compile_def = tDefine"compile"`
   (compile (Lit (StrLit s)) =
     Op (Cons string_tag) (REVERSE (MAP (λc. Op (Const (& ORD c)) []) s))) ∧
   (compile (Con cn es) =
-    Op (Cons (cn + pat_tag_shift)) (REVERSE (MAP compile es))) ∧
+    Op (Cons cn) (REVERSE (MAP compile es))) ∧
   (compile (Var_local n) =
     Var n) ∧
   (compile (Var_global n) =
@@ -45,12 +45,12 @@ val compile_def = tDefine"compile"`
   (compile (App (Op (Op (Opn Divide))) es) =
     Let (REVERSE (MAP compile es))
       (If (Op Equal [Var 0; Op (Const 0) []])
-          (Raise (Op (Cons (div_tag+pat_tag_shift)) []))
+          (Raise (Op (Cons div_tag) []))
           (Op Div [Var 0; Var 1]))) ∧
   (compile (App (Op (Op (Opn Modulo))) es) =
     Let (REVERSE (MAP compile es))
       (If (Op Equal [Var 0; Op (Const 0) []])
-          (Raise (Op (Cons (div_tag+pat_tag_shift)) []))
+          (Raise (Op (Cons div_tag) []))
           (Op Mod [Var 0; Var 1]))) ∧
   (compile (App (Op (Op (Opb Lt))) es) =
     Op Less (REVERSE (MAP compile es))) ∧
@@ -84,32 +84,32 @@ val compile_def = tDefine"compile"`
   (compile (App (Op (Op Chr)) es) =
     Let (REVERSE (MAP compile es))
       (If (Op Less [Op (Const 0) []; Var 0])
-        (Raise (Op (Cons (chr_tag+pat_tag_shift)) []))
+        (Raise (Op (Cons chr_tag) []))
         (If (Op Less [Var 0; Op (Const 255) []])
-          (Raise (Op (Cons (chr_tag+pat_tag_shift)) []))
+          (Raise (Op (Cons chr_tag) []))
           (Var 0)))) ∧
   (compile (App (Op (Op Aw8alloc)) es) =
     Let (REVERSE (MAP compile es))
       (If (Op Less [Op (Const 0) []; Var 1])
-          (Raise (Op (Cons (subscript_tag+pat_tag_shift)) []))
+          (Raise (Op (Cons subscript_tag) []))
           (Op RefByte [Var 0; Var 1]))) ∧
   (compile (App (Op (Op Aw8sub)) es) =
     Let (REVERSE (MAP compile es))
       (If (Op Less [Op (Const 0) []; Var 0])
-          (Raise (Op (Cons (subscript_tag+pat_tag_shift)) []))
+          (Raise (Op (Cons subscript_tag) []))
           (If (Op Less [Op LengthByte [Var 1]; Var 0])
               (Op DerefByte [Var 0; Var 1])
-              (Raise (Op (Cons (subscript_tag+pat_tag_shift)) []))))) ∧
+              (Raise (Op (Cons subscript_tag) []))))) ∧
   (compile (App (Op (Op Aw8length)) es) =
     Op LengthByte (REVERSE (MAP compile es))) ∧
   (compile (App (Op (Op Aw8update)) es) =
     Let (REVERSE (MAP compile es))
       (If (Op Less [Op (Const 0) []; Var 1])
-          (Raise (Op (Cons (subscript_tag+pat_tag_shift)) []))
+          (Raise (Op (Cons subscript_tag) []))
           (If (Op Less [Op LengthByte [Var 2]; Var 1])
               (Let [Op UpdateByte [Var 0; Var 1; Var 2]]
-                 (Op (Cons (tuple_tag+pat_tag_shift)) []))
-              (Raise (Op (Cons (subscript_tag+pat_tag_shift)) []))))) ∧
+                 (Op (Cons tuple_tag) []))
+              (Raise (Op (Cons subscript_tag) []))))) ∧
   (compile (App (Op (Op Explode)) es) =
     Op ToList (REVERSE (MAP compile es))) ∧
   (compile (App (Op (Op Implode)) es) =
@@ -121,41 +121,41 @@ val compile_def = tDefine"compile"`
   (compile (App (Op (Op Vsub)) es) =
     Let (REVERSE (MAP compile es))
       (If (Op Less [Op (Const 0) []; Var 0])
-          (Raise (Op (Cons (subscript_tag+pat_tag_shift)) []))
+          (Raise (Op (Cons subscript_tag) []))
           (If (Op Less [Op LengthBlock [Var 1]; Var 0])
               (Op El [Var 0; Var 1])
-              (Raise (Op (Cons (subscript_tag+pat_tag_shift)) []))))) ∧
+              (Raise (Op (Cons subscript_tag) []))))) ∧
   (compile (App (Op (Op Vlength)) es) =
     Op LengthBlock (REVERSE (MAP compile es))) ∧
   (compile (App (Op (Op Aalloc)) es) =
     Let (REVERSE (MAP compile es))
       (If (Op Less [Op (Const 0) []; Var 1])
-          (Raise (Op (Cons (subscript_tag+pat_tag_shift)) []))
+          (Raise (Op (Cons subscript_tag) []))
           (Op RefArray [Var 0; Var 1]))) ∧
   (compile (App (Op (Op Asub)) es) =
     Let (REVERSE (MAP compile es))
       (If (Op Less [Op (Const 0) []; Var 0])
-          (Raise (Op (Cons (subscript_tag+pat_tag_shift)) []))
+          (Raise (Op (Cons subscript_tag) []))
           (If (Op Less [Op Length [Var 1]; Var 0])
               (Op Deref [Var 0; Var 1])
-              (Raise (Op (Cons (subscript_tag+pat_tag_shift)) []))))) ∧
+              (Raise (Op (Cons subscript_tag) []))))) ∧
   (compile (App (Op (Op Alength)) es) =
     Op Length (REVERSE (MAP compile es))) ∧
   (compile (App (Op (Op Aupdate)) es) =
     Let (REVERSE (MAP compile es))
       (If (Op Less [Op (Const 0) []; Var 1])
-          (Raise (Op (Cons (subscript_tag+pat_tag_shift)) []))
+          (Raise (Op (Cons subscript_tag) []))
           (If (Op Less [Op Length [Var 2]; Var 1])
               (Let [Op Update [Var 0; Var 1; Var 2]]
-                 (Op (Cons (tuple_tag+pat_tag_shift)) []))
-              (Raise (Op (Cons (subscript_tag+pat_tag_shift)) []))))) ∧
+                 (Op (Cons tuple_tag) []))
+              (Raise (Op (Cons subscript_tag) []))))) ∧
   (compile (App (Op (Op (FFI n))) es) =
     Op (FFI n) (REVERSE (MAP compile es))) ∧
   (compile (App (Op (Init_global_var n)) es) =
     Let [Op (SetGlobal n) (REVERSE (MAP compile es))]
-      (Op (Cons (tuple_tag+pat_tag_shift)) [])) ∧
+      (Op (Cons tuple_tag) [])) ∧
   (compile (App (Tag_eq n l) es) =
-    Op (TagLenEq (n+pat_tag_shift) l) (REVERSE (MAP compile es))) ∧
+    Op (TagLenEq n l) (REVERSE (MAP compile es))) ∧
   (compile (App (El n) es) =
     (* TODO: check if this if is really necessary *)
     if LENGTH es ≠ 1 then Op Sub (REVERSE (MAP compile es)) else
@@ -170,7 +170,7 @@ val compile_def = tDefine"compile"`
     Letrec 0 [] (MAP (λe. (1,compile e)) es) (compile e)) ∧
   (compile (Extend_global n) =
    Let (REPLICATE n (Op AllocGlobal []))
-     (Op (Cons (tuple_tag+pat_tag_shift)) []))`
+     (Op (Cons tuple_tag) []))`
   let
     val exp_size_def = patLangTheory.exp_size_def
   in
